update arity checks

foformulas_ar.v
@@ -1,6 +1,8 @@
 (* First-Order Formulas *)
 
-Require Export foterms.
+(* with arity checks *)
+
+Require Export foterms_ar.
 
 Set Implicit Arguments.
 
@@ -10,10 +12,10 @@ Set Implicit Arguments.
 
 Section Formulas.
 
-Context { vatom : DecType } { tatom : Type }.
-Notation term := (@term vatom tatom).
-Arguments evar _ _ {T}.
-Notation evar := (evar vatom tatom).
+Context { vatom : DecType } { tatom : Type } { tarity : tatom -> nat }.
+Notation term := (@term vatom tatom tarity).
+Arguments evar _ _ _ {T}.
+Notation evar := (evar vatom tatom tarity).
 
 Notation "r ;; s" := (fecomp r s) (at level 20, format "r  ;;  s").
 Notation closed t := (tvars t = nil).
@@ -42,6 +44,7 @@ Hint Resolve tesubs_ext : term_db.
 Hint Resolve closed_notvars : term_db.
 
 Context { fatom : Type }.  (* relation symbols for [formula] *)
+Context { farity : fatom -> nat }.  (* arity of relation symbols *)
 (* Generic sets of connectives *)
 Context { NCon : Type }. (* nullary connectives *)
 Context { BCon : Type }. (* binary connectives *)
@@ -49,16 +52,18 @@ Context { QCon : Type }. (* quantifiers *)
 
 (** formulas *)
 (** first-order formulas *)
-Inductive formula T :=
-| fvar : fatom -> list (term T)-> formula T
-| fnul : NCon -> formula T
-| fbin : BCon -> formula T -> formula T -> formula T
-| fqtf : QCon -> vatom -> formula T -> formula T.
+Inductive formula T : nat -> Type :=
+| frel : forall X, formula T (farity X)
+| fconstr : forall (t : term T 0) {k}, formula T (S k) -> formula T k
+| fnul : NCon -> formula T 0
+| fbin : BCon -> formula T 0 -> formula T 0 -> formula T 0
+| fqtf : QCon -> vatom -> formula T 0 -> formula T 0.
+Arguments frel {T} _.
 Arguments fnul {T} _.
 (* Nullary connectives in [NCon] and [fnul] are mostly redundant with [fvar f nil] *)
 
 Ltac formula_induction A :=
-  (try intros until A) ;
+  try (intros until A); (* to avoid name clashes in induction t *)
   let XX := fresh "X" in
   let xx := fresh "x" in
   let ncon := fresh "ncon" in
@@ -66,27 +71,25 @@ Ltac formula_induction A :=
   let qcon := fresh "qcon" in
   let A1 := fresh A in
   let A2 := fresh A in
-  let ll := fresh "l" in
+  let BB := fresh "B" in
   let lll := fresh "l" in
   let tt := fresh "t" in
-  let IHll := fresh "IHl" in
-  induction A as [ XX ll | ncon | bcon A1 ? A2 ? | qcon xx A ]; simpl; intros;
-  [ rewrite ? flat_map_concat_map;
-    try (apply (f_equal (fvar _)));
-    try (induction ll as [ | tt lll IHll ]; simpl; intuition;
-         rewrite IHll; f_equal; intuition)
+  induction A as [ XX | tt BB | ncon | bcon A1 ? A2 ? | qcon xx A ]; simpl; intros;
+  [ try ((try f_equal); intuition; fail)
+  | try (apply (f_equal2 (fun x y => fconstr x y))); intuition
   | try ((try f_equal); intuition; fail)
   | try (apply (f_equal2 (fbin _))); intuition
-  | (try apply (f_equal (fqtf _ _))); repeat case_analysis; try (intuition; fail); 
+  | (try apply (f_equal (fqtf _ _))); repeat case_analysis; try (intuition; fail);
      try (now rcauto) ];
   try (now rcauto).
 
 
 (** * Size of [formula] *)
 
-Fixpoint fsize T (A : formula T) :=
+Fixpoint fsize T k (A : formula T k) :=
 match A with
-| fvar _ _ => 1
+| frel _ => 1
+| fconstr _ _ => 1
 | fnul _ => 1
 | fbin _ B C => S (fsize B + fsize C)
 | fqtf _ _ B => S (fsize B)
@@ -97,32 +100,33 @@ end.
 
 (** substitutes the [term] [r n] for index [n] in [formula] [A] *)
 (* capture is not avoided *)
-Fixpoint esubs T1 T2 (r : T1 -> term T2) (A : formula T1) :=
+Fixpoint esubs T1 T2 k (r : T1 -> term T2 0) (A : formula T1 k) : formula T2 k :=
 match A with
-| fvar X l => fvar X (map (tesubs r) l)
+| frel X => frel X
+| fconstr t B => fconstr ((tesubs r) t) (esubs r B)
 | fnul ncon => fnul ncon
 | fbin bcon B C => fbin bcon (esubs r B) (esubs r C)
 | fqtf qcon x B => fqtf qcon x (esubs r B)
 end.
 Notation "A ⟦ r ⟧" := (esubs r A) (at level 8, left associativity, format "A ⟦ r ⟧").
 
-Lemma fsize_esubs T1 T2 : forall (r : T1 -> term T2) A, fsize A⟦r⟧ = fsize A.
+Lemma fsize_esubs T1 T2 k : forall (r : T1 -> term T2 0) (A : formula T1 k), fsize A⟦r⟧ = fsize A.
 Proof. formula_induction A. Qed.
 Hint Rewrite fsize_esubs : term_db.
 
-Lemma esubs_evar T : forall (A : formula T),
+Lemma esubs_evar T k : forall (A : formula T k),
   A⟦evar⟧ = A.
 Proof. formula_induction A. Qed.
 Hint Rewrite esubs_evar : term_db.
 
-Lemma esubs_comp T1 T2 T3 (r : T1 -> term T2) (s : T2 -> term T3) :
-  forall A, A⟦r⟧⟦s⟧ = A⟦r ;; s⟧.
+Lemma esubs_comp T1 T2 T3 k (r : T1 -> term T2 0) (s : T2 -> term T3 0) :
+  forall A : formula T1 k, A⟦r⟧⟦s⟧ = A⟦r ;; s⟧.
 Proof. formula_induction A. Qed.
 Hint Rewrite esubs_comp : term_db.
 
 (* the result of substitution depends extensionnaly on the substituting function *)
-Lemma esubs_ext T1 T2 (r1 r2 : T1 -> term T2) :
-  r1 == r2 -> forall A, A⟦r1⟧ = A⟦r2⟧.
+Lemma esubs_ext T1 T2 k (r1 r2 : T1 -> term T2 0) :
+  r1 == r2 -> forall A : formula T1 k, A⟦r1⟧ = A⟦r2⟧.
 Proof. formula_induction A. Qed.
 
 
@@ -130,25 +134,26 @@ Proof. formula_induction A. Qed.
 
 (** substitutes [term] [u] for variable [x] in [formula] [A] *)
 (* capture is not avoided *)
-Fixpoint subs T x u (A : formula T) :=
+Fixpoint subs T k x u (A : formula T k) : formula T k :=
 match A with
-| fvar X l => fvar X (map (tsubs x u) l)
+| frel X => frel X
+| fconstr t B => fconstr (tsubs x u t) (subs x u B)
 | fnul ncon => fnul ncon
 | fbin bcon B C => fbin bcon (subs x u B) (subs x u C)
 | fqtf qcon y B => fqtf qcon y (if (eqb y x) then B else subs x u B)
 end.
 Notation "A [ u // x ]" := (subs x u A) (at level 8, format "A [ u // x ]").
 
-Lemma fsize_subs T : forall u x (A : formula T), fsize A[u//x] = fsize A.
+Lemma fsize_subs T k : forall u x (A : formula T k), fsize A[u//x] = fsize A.
 Proof. formula_induction A. Qed.
 Hint Rewrite fsize_subs : term_db.
 
 
 (** * Additional results with variable eigen type *)
 
-Lemma subs_esubs T1 T2 (r : T1 -> term T2): forall x u A, (forall n, closed (r n)) ->
-  A[u//x]⟦r⟧ = A⟦r⟧[tesubs r u//x].
-Proof. formula_induction A; simpl in H; rcauto. Qed.
+Lemma subs_esubs T1 T2 k (r : T1 -> term T2 0): forall x u (A : formula T1 k),
+  (forall n, closed (r n)) -> A[u//x]⟦r⟧ = A⟦r⟧[tesubs r u//x].
+Proof. formula_induction A. Qed.
 Hint Rewrite subs_esubs using intuition; fail : term_db.
 
 
@@ -158,11 +163,11 @@ Hint Rewrite subs_esubs using intuition; fail : term_db.
 Notation "A ↑" := (A⟦⇑⟧) (at level 8, format "A ↑").
 Notation "v ⇓" := (fesubs v) (at level 18, format "v ⇓").
 
-Lemma esubs_fup v A : A↑⟦v⇓⟧ = A.
+Lemma esubs_fup k v (A : formula nat k) : A↑⟦v⇓⟧ = A.
 Proof. rcauto. Qed.
 Hint Rewrite esubs_fup : term_db.
 
-Lemma felift_esubs u r : forall A, A⟦r⟧↑ = A↑⟦⇑[u]r⟧.
+Lemma felift_esubs k u r : forall A : formula nat k, A⟦r⟧↑ = A↑⟦⇑[u]r⟧.
 Proof. rcauto. Qed.
 Hint Rewrite felift_esubs : term_db.
 
@@ -180,7 +185,7 @@ Notation exs := (fqtf exs_con).
 
 
 Ltac formula_induction A :=
-  (try intros until A) ;
+  try (intros until A); (* to avoid name clashes in induction t *)
   let XX := fresh "X" in
   let xx := fresh "x" in
   let ncon := fresh "ncon" in
@@ -188,17 +193,14 @@ Ltac formula_induction A :=
   let qcon := fresh "qcon" in
   let A1 := fresh A in
   let A2 := fresh A in
-  let ll := fresh "l" in
+  let BB := fresh "B" in
   let lll := fresh "l" in
   let tt := fresh "t" in
-  let IHll := fresh "IHl" in
-  induction A as [ XX ll | ncon | bcon A1 ? A2 ? | qcon xx A ]; simpl; intros;
-  [ rewrite ? flat_map_concat_map;
-    try (apply (f_equal (fvar _)));
-    try (induction ll as [ | tt lll IHll ]; simpl; intuition;
-         rewrite IHll; f_equal; intuition)
+  induction A as [ XX | tt BB | ncon | bcon A1 ? A2 ? | qcon xx A ]; simpl; intros;
+  [ try ((try f_equal); intuition; fail)
+  | try (apply (f_equal2 (fun x y => fconstr x y))); intuition
   | try ((try f_equal); intuition; fail)
   | try (apply (f_equal2 (fbin _))); intuition
-  | (try apply (f_equal (fqtf _ _))); repeat case_analysis; try (intuition; fail); 
+  | (try apply (f_equal (fqtf _ _))); repeat case_analysis; try (intuition; fail);
      try (now rcauto) ];
   try (now rcauto).
