foterms_ar.v
@@ -1,0 +1,271 @@
+(* Definitions and Properties of First-Order Terms *)
+(*   with holes in [nat] for de Bruijn indices *)
+
+(* with arity checks *)
+
+From Coq Require Export PeanoNat List.
+From OLlibs Require Import List_more.
+From OLlibs Require Export dectype.
+
+Require Export term_tactics.
+
+Set Implicit Arguments.
+
+(* Extensional equality of functions *)
+Infix "==" := (fun f g => forall x, f x = g x) (at level 70).
+
+
+(** * First-Order Terms *)
+
+Section Terms.
+
+Context { vatom : DecType } { tatom : Type }.
+Context { tarity : tatom -> nat }. (* arity of function symbols *)
+
+(** terms with quantifiable variables
+
+    arity not given meaning that we have a copy of each function name for each arity
+
+ - [evar] for De Bruijn style eigen variables in proofs,
+             type for these indices as parameter called the eigen type,
+             but mostly used with [nat].
+             Other values can be used (for terms without indices, use [Empty_set]).
+ - [tvar] for quantified variables in formulas *)
+Inductive term T : nat -> Type :=
+| evar : T -> term T 0
+| tvar : vatom -> term T 0
+| tfun : forall f, term T (tarity f)
+| tconstr : forall (t : term T 0) {k}, term T (S k) -> term T k.
+Arguments evar {T}.
+Arguments tfun {T}.
+
+Ltac term_induction t :=
+  try (intros until t); (* to avoid name clashes in induction t *)
+  let nn := fresh "n" in
+  let xx := fresh "x" in
+  let ff := fresh "f" in
+  let kk := fresh "k" in
+  let uu := fresh "u" in
+  let ll := fresh "l" in
+  let IHuu := fresh "IHu" in
+  let IHll := fresh "IHl" in
+  induction t as [nn | xx | ff | uu IHuu kk ll IHll]; try (now intuition); simpl; intros;
+  try (apply (f_equal2 (fun x y => tconstr x y)); try (now intuition));
+  try (now rcauto);
+  try (now f_equal; rcauto).
+
+
+(** * Monad structure on [term] via substitution *)
+
+(** substitutes the [term] [r n] for index [n] in [term] [t] *)
+Fixpoint tesubs T1 T2 k (r : T1 -> term T2 0) (t : term T1 k) :=
+match t with
+| tvar _ x => tvar T2 x
+| evar k => r k
+| tfun f => tfun f
+| tconstr u v => tconstr (tesubs r u) (tesubs r v)
+end.
+Notation "t ⟦ r ⟧" := (tesubs r t) (at level 8, left associativity, format "t ⟦ r ⟧").
+
+(** monad structure induced on [term] *)
+Lemma evar_tesubs T1 T2 (r : T1 -> term T2 0) :
+  forall x, (evar x)⟦r⟧ = r x.
+Proof. reflexivity. Qed.
+Hint Rewrite evar_tesubs : term_db.
+
+Lemma tesubs_evar T k : forall (t : term T k),
+  t⟦evar⟧ = t.
+Proof. term_induction t. Qed.
+Hint Rewrite tesubs_evar : term_db.
+
+Definition fecomp T1 T2 T3 (r : T1 -> term T2 0) (s : T2 -> term T3 0) := fun x => (r x)⟦s⟧.
+Notation "r ;; s" := (fecomp r s) (at level 20, format "r  ;;  s").
+
+Lemma tesubs_comp T1 T2 T3 k (r : T1 -> term T2 0) (s : T2 -> term T3 0) :
+  forall t : term T1 k, t⟦r⟧⟦s⟧ = t⟦r ;; s⟧.
+Proof. term_induction t. Qed.
+Hint Rewrite tesubs_comp : term_db.
+
+(* the result of substitution depends extensionnaly on the substituting function *)
+Lemma tesubs_ext T1 T2 k (r1 r2 : T1 -> term T2 0) :
+  r1 == r2 -> forall t : term T1 k, t⟦r1⟧ = t⟦r2⟧.
+Proof. term_induction t. Qed.
+Hint Resolve tesubs_ext : term_db.
+(* TODO could be turned into a morphism *)
+
+
+Section Fixed_Eigen_Type.
+
+Variable T : Type.
+Implicit Type t : term T 0.
+Arguments tvar {T} _.
+
+(** * Term substitution *)
+
+(** substitutes [term] [u] for variable [x] in [term] [t] *)
+Fixpoint tsubs k x u (t : term T k) :=
+match t with
+| tvar y => if (eqb y x) then u else tvar y
+| evar k => evar k
+| tfun f => tfun f
+| tconstr v l => tconstr (tsubs x u v) (tsubs x u l)
+end.
+Notation "t [ u // x ]" := (tsubs x u t) (at level 8, format "t [ u // x ]").
+
+Lemma tsubs_tsubs_eq : forall x u v t, t[v//x][u//x] = t[v[u//x]//x].
+Proof. term_induction t. Qed.
+Hint Rewrite tsubs_tsubs_eq : term_db.
+
+
+(** * Variables *)
+
+Fixpoint tvars k (t : term T k) :=
+match t with
+| tvar x => x :: nil
+| evar _ => nil
+| tfun _ => nil
+| tconstr v l => tvars l ++ tvars v
+end.
+Notation "x ∈ t" := (In x (tvars t)) (at level 30).
+Notation "x ∉ t" := (~ In x (tvars t)) (at level 30).
+Notation closed t := (tvars t = nil).
+Notation fclosed r := (forall n, closed (r n)).
+
+Lemma closed_notvars : forall t x, closed t -> x ∉ t.
+Proof. intros t x Hc Hin ; now rewrite Hc in Hin. Qed.
+Hint Resolve closed_notvars : term_db.
+
+Lemma tvars_tsubs_closed : forall x u, closed u -> forall t,
+  tvars t[u//x] = remove eq_dt_dec x (tvars t).
+Proof. term_induction t; rewrite remove_app; f_equal; intuition. Qed.
+Hint Rewrite tvars_tsubs_closed using intuition; fail : term_db.
+
+Lemma notin_tsubs : forall x u t, x ∉ t -> t[u//x] = t.
+Proof. term_induction t. Qed.
+Hint Rewrite notin_tsubs using try easy;
+                              (try (intuition; fail));
+                              (try apply closed_notvars); intuition; fail : term_db.
+
+Lemma tsubs_tsubs: forall x v y u, x <> y -> x ∉ u -> forall t,
+  t[v//x][u//y] = t[u//y][v[u//y]//x].
+Proof. term_induction t. Qed.
+Hint Rewrite tsubs_tsubs using try (intuition; fail);
+                              (try apply closed_notvars); intuition; fail : term_db.
+
+Lemma notin_tsubs_bivar : forall x y t, x ∉ t -> t[tvar x//y][tvar y//x] = t.
+Proof. term_induction t. Qed.
+Hint Rewrite notin_tsubs_bivar using try easy;
+                                    (try (intuition; fail));
+                                    (try apply closed_notvars); intuition; fail : term_db.
+
+End Fixed_Eigen_Type.
+
+
+Section Two_Eigen_Types.
+
+Variable T1 T2 : Type.
+Variable r : T1 -> term T2 0.
+
+Notation closed t := (tvars t = nil).
+Notation fclosed := (forall n, closed (r n)).
+Notation "t [ u // x ]" := (tsubs x u t) (at level 8, format "t [ u // x ]").
+
+Hint Rewrite notin_tsubs using try easy;
+                              (try (intuition; fail));
+                              (try apply closed_notvars); intuition; fail : term_db.
+
+(** * Additional results with variable eigen type *)
+
+Lemma tvars_tesubs_fclosed : fclosed -> forall k (t : term T1 k), tvars t⟦r⟧ = tvars t.
+Proof. term_induction t. Qed.
+Hint Rewrite tvars_tesubs_fclosed using intuition; fail : term_db.
+
+Lemma tsubs_tesubs : forall x u k (t : term T1 k), fclosed ->
+  t[u//x]⟦r⟧ = t⟦r⟧[u⟦r⟧//x].
+Proof. term_induction t. Qed.
+Hint Rewrite tsubs_tesubs using intuition; fail : term_db.
+
+End Two_Eigen_Types.
+
+
+(* We restrict to [term nat] *)
+Section Eigen_nat.
+
+Hint Rewrite tvars_tesubs_fclosed using intuition; fail : term_db.
+
+Notation term := (term nat).
+Notation tvar := (tvar nat).
+Notation "t [ u // x ]" := (tsubs x u t) (at level 8, format "t [ u // x ]").
+Notation "x ∈ t" := (In x (tvars t)) (at level 30).
+Notation "x ∉ t" := (~ In x (tvars t)) (at level 30).
+Notation closed t := (tvars t = nil).
+Notation fclosed r := (forall n, closed (r n)).
+
+Definition fup := fun n => evar (S n).
+Notation "⇑" := fup.
+Notation "t ↑" := (t⟦⇑⟧) (at level 8, format "t ↑").
+
+Lemma fclosed_fup : fclosed ⇑.
+Proof. reflexivity. Qed.
+Hint Rewrite fclosed_fup : term_db.
+
+Lemma tvars_fup : forall k (t : term k), tvars t↑ = tvars t.
+Proof. rcauto. Qed.
+Hint Rewrite tvars_fup : term_db.
+
+Definition fesubs v := fun n =>
+  match n with
+  | 0 => v
+  | S n => evar n
+  end.
+Notation "v ⇓" := (fesubs v) (at level 18, format "v ⇓").
+
+Lemma fclosed_fesubs : forall v, closed v -> fclosed (v⇓).
+Proof. intros v Hc n; now destruct n. Qed.
+Hint Resolve fclosed_fesubs : term_db.
+
+Lemma fesubs_fup v : ⇑ ;; v⇓ == evar.
+Proof. intros ?; reflexivity. Qed.
+
+Lemma tesubs_fup v k (t : term k) : t↑⟦v⇓⟧ = t.
+Proof. rcauto. Qed.
+Hint Rewrite tesubs_fup : term_db.
+
+(* In practive only the case [u = evar 0] will be used *)
+Definition felift u (r : _ -> term 0) := fun n =>
+  match n with
+  | 0 => u
+  | S k => (r k)↑
+  end.
+Notation "⇑[ u ] r" := (felift u r) (at level 25, format "⇑[ u ] r").
+
+Lemma fclosed_felift u r : closed u -> fclosed r -> fclosed (⇑[u]r).
+Proof. intros ? ? n; rnow destruct n. Qed.
+Hint Resolve fclosed_felift : term_db.
+
+Lemma felift_comp u r : r ;; ⇑ == ⇑ ;; ⇑[u]r.
+Proof. intros ?; reflexivity. Qed.
+Hint Rewrite felift_comp : term_db.
+
+Lemma felift_tesubs u r : forall k (t : term k), t⟦r⟧↑ = t↑⟦⇑[u]r⟧.
+Proof. rcauto. Qed.
+Hint Rewrite felift_tesubs : term_db.
+
+End Eigen_nat.
+
+End Terms.
+
+Ltac term_induction t :=
+  try (intros until t); (* to avoid name clashes in induction t *)
+  let nn := fresh "n" in
+  let xx := fresh "x" in
+  let ff := fresh "f" in
+  let kk := fresh "k" in
+  let uu := fresh "u" in
+  let ll := fresh "l" in
+  let IHuu := fresh "IHu" in
+  let IHll := fresh "IHl" in
+  induction t as [nn | xx | ff | uu IHuu kk ll IHll]; try (now intuition); simpl; intros;
+  try (apply (f_equal2 (fun x y => tconstr x y)); try (now intuition));
+  try (now rcauto);
+  try (now f_equal; rcauto).
