nj1_frl_ar.v
@@ -1,0 +1,273 @@
+(* Natural Deduction for First-Order Intuitionistic Logic *)
+
+From Coq Require Import Wf_nat Lia.
+From OLlibs Require Import List_more.
+Require Export foformulas_ar.
+
+Set Implicit Arguments.
+
+
+(** * Proofs *)
+
+Section Proofs.
+
+Context { vatom : DecType } { tatom fatom : Type }.
+Context { tarity : tatom -> nat } { farity : fatom -> nat }.
+
+Arguments tvar {_} {_} {_} {T} _.
+
+Notation term := (@term vatom tatom tarity nat).
+Notation closed t := (tvars t = nil).
+Notation fclosed r := (forall n, closed (r n)).
+Notation "↑ r" := (felift (evar 0) r) (at level 25, format "↑ r").
+Notation "v ⇓" := (fesubs v) (at level 18, format "v ⇓").
+Notation "A ⟦ r ⟧" := (esubs r A) (at level 8, left associativity, format "A ⟦ r ⟧").
+Notation "A [ u // x ]" := (subs x u A) (at level 8, format "A [ u // x ]").
+Notation "⇑" := fup.
+Notation "A ↑" := (A⟦⇑⟧) (at level 8, format "A ↑").
+Notation "l ⇈" := (map (fun F => F↑) l) (at level 8, format "l ⇈").
+
+Inductive FQcon := frl_con.
+Notation frl := (fqtf frl_con).
+
+Notation formula := (@formula vatom tatom tarity fatom farity Nocon Icon FQcon nat 0).
+
+Hint Rewrite (@fsize_esubs vatom tatom tarity fatom farity Nocon Icon FQcon) : term_db.
+Hint Rewrite (@fsize_subs vatom tatom tarity fatom farity Nocon Icon FQcon nat) : term_db.
+Hint Rewrite (@tvars_tesubs_fclosed vatom tatom tarity) using intuition; fail : term_db.
+Hint Rewrite (@subs_esubs vatom tatom tarity fatom farity Nocon Icon FQcon nat)
+                         using intuition; fail : term_db.
+Hint Rewrite <- (@felift_esubs vatom tatom tarity fatom farity Nocon Icon FQcon) : term_db.
+Hint Rewrite (@esubs_fup vatom tatom tarity fatom farity Nocon Icon FQcon) : term_db.
+
+Hint Resolve fclosed_felift : term_db.
+Hint Resolve fclosed_fesubs : term_db.
+
+
+(** Proofs *)
+Inductive prove : list formula -> formula -> Type :=
+| ax : forall l1 l2 A, prove (l1 ++ A :: l2) A
+| impi l A B : prove (A :: l) B -> prove l (imp A B)
+| impe l B : forall A, prove l (imp A B) -> prove l A -> prove l B
+| frli x l A : prove l⇈ A↑[evar 0//x] -> prove l (frl x A)
+| frle x l A : forall u, closed u -> prove l (frl x A) -> prove l (subs x u A).
+Hint Constructors prove : term_db.
+Global Arguments impe { l B }.
+
+(* This [weakening] lemma is not required in the development, see rather [rweakening] below *)
+(* It is given here for comparison with alternative formalizations of Natural Deduction *)
+Lemma weakening : forall l A, prove l A -> forall l0, prove (l ++ l0) A.
+Proof.
+intros l A pi; induction pi; intros; subst;
+  try (econstructor; rewrite_all map_app; rewrite ? app_comm_cons; intuition; fail).
+rewrite <- app_assoc, <- app_comm_cons; intuition.
+Qed.
+(* an alternative slightly more general statement:
+Lemma weakening_middle : forall l A,
+  prove l A -> forall l0 l1 l2, l = l1 ++ l2 -> prove (l1 ++ l0 ++ l2) A.
+Proof.
+intros l A pi; induction pi; intros; subst;
+  try (econstructor; rewrite_all map_app; rewrite ? app_comm_cons; intuition; fail).
+destruct (elt_eq_app _ _ _ _ _ H) as [ [? [? ?]] | [? [? ?]] ]; subst;
+  rewrite ? (app_assoc _ _ (A::_)), <- ? (app_assoc _ (A::_)), <- ? app_comm_cons;
+  intuition.
+Qed.
+*)
+
+
+(** Normal Forms *)
+Inductive nprove : list formula -> formula -> Type := (* neutral terms *)
+| nax : forall l1 l2 A, nprove (l1 ++ A :: l2) A
+| nimpe l B : forall A, nprove l (imp A B) -> rprove l A -> nprove l B
+| nfrle x l A : forall u, closed u -> nprove l (frl x A) -> nprove l (subs x u A)
+with rprove : list formula -> formula -> Type := (* normal forms *)
+| rninj l A : nprove l A -> rprove l A
+| rimpi l A B : rprove (A :: l) B -> rprove l (imp A B)
+| rfrli x l A : rprove l⇈ A↑[evar 0//x] -> rprove l (frl x A).
+Hint Constructors nprove rprove : term_db.
+Global Arguments rfrli { x l A }.
+Global Arguments nimpe { l B }.
+
+Scheme nrprove_rect := Induction for nprove Sort Type
+  with rnprove_rect := Induction for rprove Sort Type.
+Combined Scheme rnprove_mutrect from nrprove_rect, rnprove_rect.
+
+Fixpoint nsize {l A} (pi : nprove l A) : nat :=
+match pi with
+| nax _ _ _  => 1
+| nimpe _ pi1 pi2 => S (nsize pi1 + rsize pi2)
+| nfrle _ _ pi0 => S (nsize pi0)
+end
+with rsize {l A} (pi : rprove l A) : nat :=
+match pi with
+| rninj pi0 => S (nsize pi0)
+| rimpi pi0 => S (rsize pi0)
+| rfrli pi0 => S (rsize pi0)
+end.
+
+Theorem denormalization :
+   (forall l A, nprove l A -> prove l A)
+ * (forall l A, rprove l A -> prove l A).
+Proof. now apply rnprove_mutrect; intros; try (econstructor; eassumption). Qed.
+
+
+(** * Normalization *)
+
+(** apply [r] on normal form *)
+Theorem rnpesubs r (Hc : fclosed r) {l A} :
+   (nprove l A -> nprove (map (esubs r) l) A⟦r⟧)
+ * (rprove l A -> rprove (map (esubs r) l) A⟦r⟧).
+Proof.
+revert l A.
+enough ((forall l A, nprove l A -> forall r, fclosed r -> nprove (map (esubs r) l) A⟦r⟧)
+      * (forall l A, rprove l A -> forall r, fclosed r -> rprove (map (esubs r) l) A⟦r⟧))
+  as He by (split; intros; apply He; assumption).
+clear r Hc; apply rnprove_mutrect; intros; (try simpl in X);
+  (try assert (IH1 := X r H)); (try assert (IH2 := X0 r H));
+  (try (econstructor; (eassumption + intuition); fail)).
+- rewrite map_app; apply nax.
+- rcauto; rnow apply nfrle.
+- specialize X with (↑r0).
+  revert X; rcauto.
+  rewrite map_map, <- (map_ext _ _ (felift_esubs (evar 0) _)), <- map_map in X; intuition.
+Qed.
+
+Lemma rpsubsz {l A x u} : closed u ->
+  rprove l⇈ A↑[evar 0//x] -> rprove l (subs x u A).
+Proof.
+intros Hc pi.
+apply (rnpesubs (u⇓)) in pi; [ | intuition ].
+rnow simpl in pi then simpl in pi.
+now rewrite map_map, (map_ext _ _ (esubs_fup _)), map_id in pi.
+Qed.
+
+Lemma rweakening :
+   (forall l A, nprove l A -> forall l0 l1 l2, l = l1 ++ l2 -> nprove (l1 ++ l0 ++ l2) A)
+ * (forall l A, rprove l A -> forall l0 l1 l2, l = l1 ++ l2 -> rprove (l1 ++ l0 ++ l2) A).
+Proof.
+apply rnprove_mutrect; intros; subst;
+  try (econstructor; rewrite_all map_app; rewrite ? app_comm_cons; intuition; fail).
+destruct (dichot_elt_app_inf _ _ _ _ _ H) as [ [? [? ?]] | [? [? ?]] ]; subst;
+  rewrite ? (app_assoc _ _ (A::_)), <- ? (app_assoc _ (A::_)), <- ? app_comm_cons;
+  intuition.
+Qed.
+
+Lemma substitution : forall l A B, rprove l A -> rprove (A :: l) B -> rprove l B.
+Proof.
+pose (IH := (fun n m =>
+ forall A, fsize A = n ->
+   (forall B l1 l2 (pi : nprove (l1 ++ A :: l2) B),
+      nsize pi < m -> fsize A < fsize B -> rprove (l1 ++ l2) A -> nprove (l1 ++ l2) B)
+ * (forall B l1 l2 (pi : nprove (l1 ++ A :: l2) B),
+      nsize pi < m -> rprove (l1 ++ l2) A -> rprove (l1 ++ l2) B)
+ * (forall B l1 l2 (pi : rprove (l1 ++ A :: l2) B),
+      rsize pi < m -> rprove (l1 ++ l2) A -> rprove (l1 ++ l2) B))).
+enough (forall n m, IH n m) as Hsub.
+{ intros l A B pi1 pi2.
+  rewrite <- (app_nil_l (A :: l)) in pi2; rewrite <- (app_nil_l l).
+  refine (snd (Hsub _ (S (rsize pi2)) _ _) _ _ _ _ _ _); intuition. }
+apply lt_wf_double_rect; unfold IH; clear IH; simpl;
+ intros n m IHn IHm A HA; (split; [ split | ] ); subst;
+ intros B l1 l2 pi2 Hpi; [ intros HF | | ]; intros pi1;
+ remember (l1 ++ A :: l2) as ll; destruct pi2; subst; simpl in Hpi.
+(* first statement *)
+- destruct (dichot_elt_app_inf _ _ _ _ _ Heqll)
+    as [ (l' & Heq0 & Heq) | (l' & Heq0 & Heq) ]; subst.
+  + rewrite <- app_assoc; apply nax.
+  + destruct l'; inversion Heq; subst.
+    * exfalso; lia.
+    * rewrite app_assoc; apply nax.
+- assert (nsize pi2 < S (nsize pi2 + rsize r)) as IH1 by lia.
+  assert (rsize r < S (nsize pi2 + rsize r)) as IH2 by lia.
+  eapply nimpe; eapply (IHm (S (nsize pi2 + rsize r))); simpl; eauto; lia.
+- apply nfrle; auto.
+  rnow eapply (IHm _ Hpi).
+(* second statement *)
+- enough (forall l l1 l2, l0 ++ A0 :: l3 = l1 ++ A :: l2 ->
+      rprove (l ++ l1 ++ l2) A -> rprove (l ++ l1 ++ l2) A0)
+    as HI by (eapply (HI nil); eassumption) ; clear.
+  induction l0; intros l l1 l2 Heq pi; destruct l1; inversion Heq; subst; auto.
+  + rewrite <- app_comm_cons; apply rninj, nax.
+  + rewrite 2 app_assoc; apply rninj, nax.
+  + rewrite <- app_comm_cons, <- (app_nil_l l1), <- app_assoc, app_comm_cons, app_assoc.
+    apply IHl0; auto.
+    now rewrite <- ? app_assoc, <- app_comm_cons.
+- assert (nsize pi2 < S (nsize pi2 + rsize r)) as IH1 by lia.
+  assert (rsize r < S (nsize pi2 + rsize r)) as IH2 by lia.
+  eapply IHm in IH2; eauto.
+  assert ({fsize (imp A0 B) <= fsize A} + {fsize A < fsize (imp A0 B)}) as [ Ho | Ho ]
+    by (case (CompareSpec2Type (Nat.compare_spec (fsize (imp A0 B)) (fsize A))); intros Ho;
+          [ left | left | right ]; lia); simpl in Ho.
+  + eapply IHm in IH1; eauto.
+    inversion_clear IH1 as [ l' A' pi1' | l' A' B' pi1' | ].
+    * apply rninj; eapply nimpe; eauto.
+    * rewrite <- (app_nil_l _) in pi1'.
+      refine (snd (IHn (fsize A0) (S (rsize pi1')) _ _ _) _ _ _ pi1' _ IH2); lia.
+  + apply rninj, (nimpe A0); auto.
+    eapply IHm; eauto; lia.
+- assert (nsize pi2 < S (nsize pi2)) as IH1 by lia.
+  apply IHm in IH1; auto.
+  inversion_clear IH1.
+  + now apply rninj, nfrle.
+  + now apply rpsubsz.
+(* third statement *)
+- refine (snd (fst (IHm _ _ _ _)) _ _ _ n _ _); auto; lia.
+- revert pi2 Hpi; rewrite app_comm_cons; intros pi2 Hpi.
+  apply rimpi.
+  refine (snd (IHm _ _ _ _) _ _ _ pi2 _ _); auto; try lia.
+  rewrite <- app_comm_cons, <- (app_nil_l (l1 ++ l2)), app_comm_cons, <- (app_nil_l _).
+  eapply rweakening; eauto.
+- apply rfrli; rewrite map_app.
+  apply (rnpesubs ⇑) in pi1; intuition.
+  revert pi1 pi2 Hpi; rewrite ? map_app; simpl; intros pi1 pi2 Hpi.
+  rnow (refine (snd (IHm _ _ _ _) _ _ _ pi2 _ _); auto).
+Qed.
+
+Theorem normalization : forall l A, prove l A -> rprove l A.
+Proof.
+intros l A pi; induction pi; try (econstructor; (idtac + econstructor); eassumption).
+- inversion_clear IHpi1.
+  + apply rninj; eapply nimpe; eassumption.
+  + eapply substitution; eassumption.
+- inversion_clear IHpi.
+  + apply rninj; now eapply nfrle.
+  + now apply rpsubsz.
+Qed.
+
+End Proofs.
+
+
+(** * Examples *)
+Section Examples.
+
+Context { vatom : DecType } { tatom fatom : Type }.
+
+Variable f : tatom.
+Variable x : vatom.
+Variable P : fatom.
+Definition tarity : tatom -> nat := fun _ => 1.
+Definition farity : fatom -> nat := fun _ => 1.
+
+Notation frl := (fqtf frl_con).
+Notation formula := (@formula vatom tatom tarity fatom farity Nocon Icon FQcon nat).
+
+Hint Rewrite (@eqb_refl vatom): term_db.
+
+(* Apply all (reversible) introduction rules *)
+Ltac rev_intros := repeat (repeat apply rimpi; repeat (apply rfrli; simpl)); apply rninj.
+
+Goal rprove nil
+  (imp (frl x (fconstr (tconstr (tvar _ x) (tfun _ f)) (frel _ P)))
+       (frl x (fconstr (tconstr (tconstr (tvar _ x) (tfun _ f))
+                                                  (tfun _ f)) (frel _ P)))).
+Proof.
+rnow rev_intros.
+replace (fconstr (k:=0) (tconstr (tconstr (evar 0) (tfun nat f)) (tfun nat f)) (frel nat P))
+   with (subs x (tconstr (evar 0) (tfun nat f))
+        (fconstr (tconstr (tvar _ x) (tfun nat f)) (frel nat P : formula 1)))
+  by rcauto.
+apply nfrle; auto.
+rewrite <- (app_nil_l (_ :: _)) ; apply nax.
+Qed.
+
+End Examples.
